theory/Sound_Communication_B.thy
@@ -83,46 +83,46 @@ inductive
   staticLiveChanEnv :: "static_env \<Rightarrow> tm_id_map \<Rightarrow> tm_id_map \<Rightarrow> name \<Rightarrow> env \<Rightarrow> bool"  and
   staticLiveChanVal :: "static_env \<Rightarrow> tm_id_map \<Rightarrow> tm_id_map \<Rightarrow> name \<Rightarrow> val \<Rightarrow> bool"
 where
-  Intro:
+  StaticLiveChanEnv:
   "
     \<forall> x \<omega> . \<rho> x = Some \<omega> \<longrightarrow>  staticLiveChanVal V Ln Lx x\<^sub>c \<omega> \<Longrightarrow>
     staticLiveChanEnv V Ln Lx x\<^sub>c \<rho>
   "
-| Unit:
+| StaticLiveChanUnit:
   "
     staticLiveChanVal V Ln Lx x\<^sub>c VUnt
   "
-| Chan:
+| StaticLiveChan:
   "
     staticLiveChanVal V Ln Lx x\<^sub>c (VChn c)
   "
-| SendEvt:
+| StaticLiveChanSendEvt:
   "
     staticLiveChanEnv V Ln Lx x\<^sub>c \<rho> \<Longrightarrow>
     staticLiveChanVal V Ln Lx x\<^sub>c (VClsr (SendEvt _ _) \<rho>)
   "
-| RecvEvt:
+| StaticLiveChanRecvEvt:
   "
     staticLiveChanEnv V Ln Lx x\<^sub>c \<rho> \<Longrightarrow>
     staticLiveChanVal V Ln Lx x\<^sub>c (VClsr (RecvEvt _) \<rho>)
   "
-| Left:
+| StaticLiveChanLeft:
   "
     staticLiveChanEnv V Ln Lx x\<^sub>c \<rho> \<Longrightarrow>
     staticLiveChanVal V Ln Lx x\<^sub>c (VClsr (Lft _) \<rho>)
   "
-| Right:
+| StaticLiveChanRight:
   "
     staticLiveChanEnv V Ln Lx x\<^sub>c \<rho> \<Longrightarrow>
     staticLiveChanVal V Ln Lx x\<^sub>c (VClsr (Rht _) \<rho>)
   "
-| Fun:
+| StaticLiveChanFun:
   "
     staticLiveChan V Ln Lx x\<^sub>c e \<Longrightarrow> 
     staticLiveChanEnv V Ln Lx x\<^sub>c \<rho> \<Longrightarrow>
     staticLiveChanVal V Ln Lx x\<^sub>c (VClsr (Fun f x e) \<rho>)
   "
-| Pair:
+| StaticLiveChanPair:
   "
     staticLiveChanEnv V Ln Lx x\<^sub>c \<rho> \<Longrightarrow>
     staticLiveChanVal V Ln Lx x\<^sub>c (VClsr (Pair _ _) \<rho>)
@@ -297,6 +297,672 @@ lemma static_equalitySound: "
 
 (* PATH SOUND *)
 
+lemma staticFlowsAcceptPoolPreservedReturnEval:
+  "
+  staticFlowsAcceptPool V F \<E>m \<Longrightarrow>
+  (V, C) \<Turnstile>\<^sub>\<E> \<E>m \<Longrightarrow>
+  leaf \<E>m pi \<Longrightarrow>
+  \<E>m pi = Some (Stt (Rslt x) env (Ctn xk ek envk # k)) \<Longrightarrow> 
+  env x = Some v \<Longrightarrow> 
+  staticFlowsAcceptPool V F (\<E>m(pi @ [LRtn x] \<mapsto> (Stt ek (envk(xk \<mapsto> v)) k)))
+"
+proof -
+assume 
+ H1: "staticFlowsAcceptPool V F \<E>m" and
+ H2: "(V, C) \<Turnstile>\<^sub>\<E> \<E>m" and
+ H3: "leaf \<E>m pi" and
+ H4: "\<E>m pi = Some (Stt (Rslt x) env (Ctn xk ek envk # k))" and
+ H5: "env x = Some v"
+
+
+ have 
+  H6: " 
+    \<forall>\<pi> e \<rho> \<kappa>.
+    \<E>m \<pi> = Some (Stt e \<rho> \<kappa>) \<longrightarrow>
+    staticFlowsAccept V F e \<and> staticFlowsAcceptEnv V F \<rho> \<and> staticFlowsAcceptStack V F (\<lfloor>e\<rfloor>) \<kappa>"
+  using H1 staticFlowsAcceptPool.cases by blast 
+
+  have 
+    H7: "staticFlowsAccept V F (Rslt x)" by (simp add: staticFlowsAccept.Result)
+  have
+     H8: "staticFlowsAcceptEnv V F env" using H4 H6 by blast
+  have
+     H9: "staticFlowsAcceptStack V F x ((Ctn xk ek envk) # k)" using H4 H6 by fastforce
+
+  have 
+    H10: "staticFlowsAccept V F ek \<and> staticFlowsAcceptEnv V F envk \<and> staticFlowsAcceptStack V F (\<lfloor>ek\<rfloor>) k" 
+    using H9 proof cases
+    case Nonempty
+    then show ?thesis by blast
+  qed
+
+
+ show "staticFlowsAcceptPool V F (\<E>m(pi @ [LRtn x] \<mapsto> (Stt ek (envk(xk \<mapsto> v)) k)))"
+   using H1 H10 H5 H8 staticFlowsAcceptEnv.simps staticFlowsAcceptPool.simps by auto
+qed
+
+
+
+lemma staticFlowsAcceptPoolPreservedSeqEval:
+  "
+  staticFlowsAcceptPool V F \<E>m \<Longrightarrow>
+  (V, C) \<Turnstile>\<^sub>\<E> \<E>m \<Longrightarrow>
+  leaf \<E>m pi \<Longrightarrow>
+  \<E>m pi = Some (Stt (Bind x b e) env k) \<Longrightarrow> 
+  seqEval b env v \<Longrightarrow> 
+  staticFlowsAcceptPool V F (\<E>m(pi @ [LNxt x] \<mapsto> (Stt e (env(x \<mapsto> v)) k)))
+"
+proof -
+  assume 
+    H1: "staticFlowsAcceptPool V F \<E>m" and
+    H2: "(V, C) \<Turnstile>\<^sub>\<E> \<E>m" and
+    H3: "leaf \<E>m pi" and
+    H4: "\<E>m pi = Some (Stt (Bind x b e) env k)" and 
+    H5: "seqEval b env v"
+
+  have H6:
+  "
+    \<forall>\<pi> e \<rho> \<kappa>.
+    \<E>m \<pi> = Some (Stt e \<rho> \<kappa>) \<longrightarrow>
+    staticFlowsAccept V F e \<and> staticFlowsAcceptEnv V F \<rho> \<and> staticFlowsAcceptStack V F (\<lfloor>e\<rfloor>) \<kappa>"
+  using H1 staticFlowsAcceptPool.cases by blast 
+
+  have 
+    H7: "staticFlowsAccept V F (Bind x b e)"
+    using H4 H6 by auto
+  have
+     H8: "staticFlowsAcceptEnv V F env"
+    using H4 H6 by blast
+  have
+     H9: "staticFlowsAcceptStack V F (\<lfloor>Bind x b e\<rfloor>) k"
+    using H4 H6 by fastforce
+
+  have H10: 
+    "staticFlowsAccept V F e" using H7 staticFlowsAccept.cases by blast
+
+  show "staticFlowsAcceptPool V F (\<E>m(pi @ [LNxt x] \<mapsto> (Stt e (env(x \<mapsto> v)) k)))"
+  using H5
+  proof cases
+    case UNIT
+    then show ?thesis
+    using H1 H10 H8 H9 staticFlowsAcceptEnv.simps 
+      staticFlowsAcceptEnv_staticFlowsAcceptVal.Unit 
+      staticFlowsAcceptPool.simps by auto
+  next
+    case (PRIM p)
+
+    have L1H1: "staticFlowsAcceptVal V F (VClsr p env)" 
+    proof (cases p)
+      case (SendEvt x11 x12)
+      then show ?thesis
+        by (simp add: H8 staticFlowsAcceptEnv_staticFlowsAcceptVal.SendEvt)
+    next
+      case (RecvEvt x2)
+      then show ?thesis
+        by (simp add: H8 staticFlowsAcceptEnv_staticFlowsAcceptVal.RecvEvt)
+    next
+      case (Pair x31 x32)
+      then show ?thesis
+        by (simp add: H8 staticFlowsAcceptEnv_staticFlowsAcceptVal.Pair)
+    next
+      case (Lft x4)
+      then show ?thesis
+        by (simp add: H8 Left)
+    next
+      case (Rht x5)
+      then show ?thesis
+        by (simp add: H8 Right)
+    next
+      case (Fun f' x' e')
+      have L2H1: "staticFlowsAccept V F (Bind x (Atom (Fun f' x' e')) e)"
+        using H7 local.Fun local.PRIM(1) by auto
+      show ?thesis using L2H1
+      proof cases
+        case BindFun
+        then show ?thesis
+        by (simp add: H8 local.Fun staticFlowsAcceptEnv_staticFlowsAcceptVal.Fun)
+      qed
+    qed
+
+    have L1H2: "staticFlowsAcceptEnv V F (env(x \<mapsto> v))"
+      using H8 L1H1 local.PRIM(2) staticFlowsAcceptEnv.simps by auto
+    show ?thesis
+      using H10 H6 H9 L1H2 staticFlowsAcceptPool.simps by auto
+  next
+    case (FST xp x1 x2 envp)
+
+    have L1H1: "staticFlowsAcceptVal V F (VClsr (atom.Pair x1 x2) envp)" 
+    using H8 staticFlowsAcceptEnv.cases
+          using FST(2) by blast
+
+    have L1H2: "staticFlowsAcceptEnv V F envp" using L1H1 
+    proof cases
+      case Pair
+      then show ?thesis by auto
+    qed
+
+    have L1H3: "staticFlowsAcceptVal V F v"
+      using L1H2 local.FST(3) staticFlowsAcceptEnv.cases by blast
+
+    have L1H4: "staticFlowsAcceptEnv V F (env(x \<mapsto> v))"
+      using H8 L1H3 staticFlowsAcceptEnv.simps by auto
+
+    show ?thesis using H10 H6 H9 L1H4 staticFlowsAcceptPool.intros by auto
+  next
+    case (SND xp x1 x2 envp)
+    have L1H1: "staticFlowsAcceptVal V F (VClsr (atom.Pair x1 x2) envp)" 
+    using H8 staticFlowsAcceptEnv.cases
+          using SND(2) by blast
+
+    have L1H2: "staticFlowsAcceptEnv V F envp" using L1H1 
+    proof cases
+      case Pair
+      then show ?thesis by auto
+    qed
+
+    have L1H3: "staticFlowsAcceptVal V F v"
+      using L1H2 SND(3) staticFlowsAcceptEnv.cases by blast
+
+    have L1H4: "staticFlowsAcceptEnv V F (env(x \<mapsto> v))"
+      using H8 L1H3 staticFlowsAcceptEnv.simps by auto
+
+    show ?thesis using H10 H6 H9 L1H4 staticFlowsAcceptPool.intros by auto
+  qed
+qed
+
+
+lemma staticFlowsAcceptPoolPreservedCallEval:
+  "
+  staticFlowsAcceptPool V F \<E>m \<Longrightarrow>
+  (V, C) \<Turnstile>\<^sub>\<E> \<E>m \<Longrightarrow>
+  leaf \<E>m pi \<Longrightarrow>
+  \<E>m pi = Some (Stt (Bind x b e) env k) \<Longrightarrow>
+  callEval (b, env) (e', env') \<Longrightarrow> 
+  staticFlowsAcceptPool V F (\<E>m(pi @ [LCall x] \<mapsto> (Stt e' env' ((Ctn x e env) # k))))
+"
+proof -
+  assume 
+    H1: "staticFlowsAcceptPool V F \<E>m" and
+    H2: "(V, C) \<Turnstile>\<^sub>\<E> \<E>m" and
+    H3: "leaf \<E>m pi" and
+    H4: "\<E>m pi = Some (Stt (Bind x b e) env k)" and
+    H5: "callEval (b, env) (e', env')"
+
+  have H6:
+  "
+    \<forall>\<pi> e \<rho> \<kappa>.
+    \<E>m \<pi> = Some (Stt e \<rho> \<kappa>) \<longrightarrow>
+    staticFlowsAccept V F e \<and> staticFlowsAcceptEnv V F \<rho> \<and> staticFlowsAcceptStack V F (\<lfloor>e\<rfloor>) \<kappa>"
+  using H1 staticFlowsAcceptPool.cases by blast 
+
+  have 
+    H7: "staticFlowsAccept V F (Bind x b e)"
+  using H4 H6 by blast
+
+  have
+     H8: "staticFlowsAcceptEnv V F env"
+    using H4 H6 by blast
+  have
+     H9: "staticFlowsAcceptStack V F (\<lfloor>Bind x b e\<rfloor>) k"
+    using H4 H6 by fastforce
+
+  have H10: 
+    "staticFlowsAccept V F e" using H7 staticFlowsAccept.cases by blast
+
+  show "staticFlowsAcceptPool V F (\<E>m(pi @ [LCall x] \<mapsto> (Stt e' env' ((Ctn x e env) # k))))"
+  using H5
+  proof cases
+    case (CaseLft xs xl' envl vl xl xr er)
+
+    have L1H1: "staticFlowsAcceptVal V F (VClsr (Lft xl') envl)"
+      using H8 local.CaseLft(3) staticFlowsAcceptEnv.cases by blast
+
+    have L1H2: "staticFlowsAcceptEnv V F envl"
+    using L1H1 
+    proof cases
+      case Left
+      then show ?thesis by auto
+    qed
+
+    have L1H3: "staticFlowsAcceptVal V F vl"
+    using L1H2  local.CaseLft(4) staticFlowsAcceptEnv.cases by blast
+
+    have L1H4: "staticFlowsAcceptEnv V F env'"
+    using H8 L1H2 local.CaseLft(2) local.CaseLft(4) staticFlowsAcceptEnv.simps by auto
+
+    have L1H5: "staticFlowsAccept V F (Bind x (Case xs xl e' xr er) e)"
+      using H7 local.CaseLft(1) by blast
+
+    have L1H6: "staticFlowsAccept V F e'"
+    using L1H5 
+    proof cases
+      case BindCase
+      then show ?thesis
+        by blast
+    qed
+
+
+    have L1H7: "{(IdRslt (\<lfloor>e'\<rfloor>), EReturn, tmId e)} \<subseteq> F" 
+    using L1H5 proof cases
+      case BindCase
+      then show ?thesis sorry
+    qed
+    have L1H8: "staticFlowsAcceptStack V F (\<lfloor>e'\<rfloor>) (Ctn x e env # k)"
+      using H10 H8 H9 L1H7 staticFlowsAcceptStack.Nonempty by auto
+
+    show ?thesis by (simp add: H6 L1H4 L1H6 L1H8 staticFlowsAcceptPool.intros)
+
+
+
+  next
+    case (CaseRht xs xr' envr vr xl el xr)
+    have L1H1: "staticFlowsAcceptVal V F (VClsr (Rht xr') envr)"
+      using H8 local.CaseRht(3) staticFlowsAcceptEnv.cases by blast
+
+    have L1H2: "staticFlowsAcceptEnv V F envr"
+    using L1H1 
+    proof cases
+      case Right
+      then show ?thesis by auto
+    qed
+
+    have L1H3: "staticFlowsAcceptVal V F vr"
+    using L1H2  local.CaseRht(4) staticFlowsAcceptEnv.cases by blast
+
+    have L1H4: "staticFlowsAcceptEnv V F env'"
+    using H8 L1H2 local.CaseRht(2) local.CaseRht(4) staticFlowsAcceptEnv.simps by auto
+
+    have L1H5: "staticFlowsAccept V F (Bind x (Case xs xl el xr e') e)"
+      using H7 local.CaseRht(1) by blast
+
+    have L1H6: "staticFlowsAccept V F e'"
+    using L1H5 
+    proof cases
+      case BindCase
+      then show ?thesis
+        by blast
+    qed
+
+    have L1H7: "{(IdRslt (\<lfloor>e'\<rfloor>), EReturn, tmId e)} \<subseteq> F" 
+    using L1H5 proof cases
+      case BindCase
+      then show ?thesis sorry
+    qed
+    have L1H8: "staticFlowsAcceptStack V F (\<lfloor>e'\<rfloor>) (Ctn x e env # k)"
+      using H10 H8 H9 L1H7 staticFlowsAcceptStack.Nonempty by auto
+
+    show ?thesis by (simp add: H6 L1H4 L1H6 L1H8 staticFlowsAcceptPool.intros)
+
+  next
+    case (App f fp xp envl xa va)
+
+    have L1H1: "staticFlowsAcceptVal V F (VClsr (Fun fp xp e') envl)"
+      using H8 local.App(3) staticFlowsAcceptEnv.cases by blast
+
+
+    have L1H2: "staticFlowsAccept V F e'"
+    using L1H1 proof cases
+      case Fun
+      then show ?thesis
+        by simp
+    qed
+
+    have L1H3: "staticFlowsAcceptEnv V F envl"
+    using L1H1 proof cases
+      case Fun
+      then show ?thesis
+        by simp
+    qed
+
+
+    have L1H4: "staticFlowsAcceptVal V F va"
+      using H8 local.App(4) staticFlowsAcceptEnv.cases by blast
+
+    have L1H5: "staticFlowsAcceptEnv V F env'"
+      using H8 L1H3 local.App(2) local.App(3) local.App(4) staticFlowsAcceptEnv.simps by auto
+
+
+    have L1H6: "staticFlowsAccept V F (Bind x (App f xa) e)" using H7 local.App(1) by auto
+
+    have L1H7: "staticFlowsAccept V F e'"
+    using L1H6
+    proof cases
+      case BindApp
+      then show ?thesis using L1H2 by blast
+    qed
+
+    have L1H7: "{(IdRslt (\<lfloor>e'\<rfloor>), EReturn, tmId e)} \<subseteq> F" 
+    using L1H6 proof cases
+      case BindApp
+      then show ?thesis
+        using H2 H4 local.App(3) staticEvalPoolSoundSnapshot sorry
+    qed
+
+    have L1H8: "staticFlowsAcceptStack V F (\<lfloor>e'\<rfloor>) (Ctn x e env # k)"
+      using H10 H8 H9 L1H7 staticFlowsAcceptStack.Nonempty by auto
+
+    show ?thesis
+      by (simp add: H6 L1H2 L1H5 L1H8 staticFlowsAcceptPool.intros)
+  qed
+qed
+
+lemma staticFlowsAcceptPoolPreservedMkChnEval:
+  "
+  staticFlowsAcceptPool V F \<E>m \<Longrightarrow>
+  (V, C) \<Turnstile>\<^sub>\<E> \<E>m \<Longrightarrow>
+  leaf \<E>m pi \<Longrightarrow> 
+  \<E>m pi = Some (Stt (Bind x MkChn e) env k) \<Longrightarrow> 
+  staticFlowsAcceptPool V F (\<E>m(pi @ [LNxt x] \<mapsto> (Stt e (env(x \<mapsto> VChn (Ch pi x))) k)))
+"
+proof -
+  assume 
+    H1: "staticFlowsAcceptPool V F \<E>m" and
+    H2: "(V, C) \<Turnstile>\<^sub>\<E> \<E>m" and
+    H3: "leaf \<E>m pi" and
+    H4: "\<E>m pi = Some (Stt (Bind x MkChn e) env k)"
+
+  have H6:
+  "
+    \<forall>\<pi> e \<rho> \<kappa>.
+    \<E>m \<pi> = Some (Stt e \<rho> \<kappa>) \<longrightarrow>
+    staticFlowsAccept V F e \<and> staticFlowsAcceptEnv V F \<rho> \<and> staticFlowsAcceptStack V F (\<lfloor>e\<rfloor>) \<kappa>"
+  using H1 staticFlowsAcceptPool.cases by blast 
+
+  have 
+    H7: "staticFlowsAccept V F (Bind x MkChn e)"
+  using H4 H6 by blast
+
+
+  have
+     H8: "staticFlowsAcceptEnv V F env"
+    using H4 H6 by blast
+  have
+     H9: "staticFlowsAcceptStack V F (\<lfloor>Bind x MkChn e\<rfloor>) k"
+    using H4 H6 by blast
+
+  have H10: 
+    "staticFlowsAccept V F e" using H7 staticFlowsAccept.cases by blast
+
+  show "staticFlowsAcceptPool V F (\<E>m(pi @ [LNxt x] \<mapsto> (Stt e (env(x \<mapsto> VChn (Ch pi x))) k)))"
+    using H10 H6 H8 H9 staticFlowsAcceptEnv.simps 
+    staticFlowsAcceptEnv_staticFlowsAcceptVal.Chan 
+    staticFlowsAcceptPool.simps by auto
+
+qed
+
+lemma staticFlowsAcceptPoolPreservedSpawnEval:
+  "
+  staticFlowsAcceptPool V F \<E>m \<Longrightarrow>
+  (V, C) \<Turnstile>\<^sub>\<E> \<E>m \<Longrightarrow>
+  leaf \<E>m pi \<Longrightarrow> 
+  \<E>m pi = Some (Stt (Bind x (Spwn ec) e) env k) \<Longrightarrow> 
+  staticFlowsAcceptPool V F (\<E>m(pi @ [LNxt x] \<mapsto> (Stt e (env(x \<mapsto> VUnt)) k), pi @ [LSpwn x] \<mapsto> (Stt ec env [])))
+"
+proof -
+  assume 
+    H1: "staticFlowsAcceptPool V F \<E>m" and
+    H2: "(V, C) \<Turnstile>\<^sub>\<E> \<E>m" and
+    H3: "leaf \<E>m pi" and
+    H4: "\<E>m pi = Some (Stt (Bind x (Spwn ec) e) env k)"
+
+  have H6:
+  "
+    \<forall>\<pi> e \<rho> \<kappa>.
+    \<E>m \<pi> = Some (Stt e \<rho> \<kappa>) \<longrightarrow>
+    staticFlowsAccept V F e \<and> staticFlowsAcceptEnv V F \<rho> \<and> staticFlowsAcceptStack V F (\<lfloor>e\<rfloor>) \<kappa>"
+  using H1 staticFlowsAcceptPool.cases by blast 
+
+  have 
+    H7: "staticFlowsAccept V F (Bind x (Spwn ec) e)"
+  using H4 H6 by blast
+
+
+  have
+     H8: "staticFlowsAcceptEnv V F env"
+    using H4 H6 by blast
+  have
+     H9: "staticFlowsAcceptStack V F (\<lfloor>Bind x (Spwn ec) e\<rfloor>) k"
+    using H4 H6 by blast
+
+  have H10: "staticFlowsAccept V F e" using H7 staticFlowsAccept.cases by blast
+
+
+  have 
+    H11: "staticFlowsAccept V F ec" using H7 staticFlowsAccept.cases by blast
+
+  have 
+    H12: "staticFlowsAcceptVal V F VUnt"
+    by (simp add: staticFlowsAcceptEnv_staticFlowsAcceptVal.Unit)
+
+  have 
+    H13: "staticFlowsAcceptStack V F (\<lfloor>Bind x (Spwn ec) e\<rfloor>) []"
+    by (simp add: staticFlowsAcceptStack.Empty) 
+
+  have H14: "staticFlowsAcceptEnv V F (env(x \<mapsto> VUnt))"
+    using H12 H8 staticFlowsAcceptEnv.simps by auto
+
+  show ?thesis
+    using H10 H11 H13 H14 H6 H8 H9 staticFlowsAcceptPool.simps by (simp add: staticFlowsAcceptStack.Empty)
+
+qed
+
+
+lemma staticFlowsAcceptPoolPreservedSyncEval:
+  "
+  staticFlowsAcceptPool V F \<E>m \<Longrightarrow>
+  (V, C) \<Turnstile>\<^sub>\<E> \<E>m \<Longrightarrow>
+  leaf \<E>m pis \<Longrightarrow>
+  \<E>m pis = Some (Stt (Bind xs (Sync xse) es) envs ks) \<Longrightarrow>
+  envs xse = Some (VClsr (SendEvt xsc xm) envse) \<Longrightarrow>
+  leaf \<E>m pir \<Longrightarrow>
+  \<E>m pir = Some (Stt (Bind xr (Sync xre) er) envr kr) \<Longrightarrow>
+  envr xre = Some (VClsr (RecvEvt xrc) envre) \<Longrightarrow>
+  envse xsc = Some (VChn c) \<Longrightarrow>
+  envre xrc = Some (VChn c) \<Longrightarrow> 
+  envse xm = Some vm \<Longrightarrow> 
+  staticFlowsAcceptPool V F 
+    (\<E>m(pis @ [LNxt xs] \<mapsto> (Stt es (envs(xs \<mapsto> VUnt)) ks), pir @ [LNxt xr] \<mapsto> (Stt er (envr(xr \<mapsto> vm)) kr)))
+"
+proof -
+  assume 
+    H1: "staticFlowsAcceptPool V F \<E>m" and
+    H2: "(V, C) \<Turnstile>\<^sub>\<E> \<E>m" and
+    H3: "leaf \<E>m pis" and
+    H4: "\<E>m pis = Some (Stt (Bind xs (Sync xse) es) envs ks)" and
+    H5: "envs xse = Some (VClsr (SendEvt xsc xm) envse)" and
+    H6: "leaf \<E>m pir" and
+    H7: "\<E>m pir = Some (Stt (Bind xr (Sync xre) er) envr kr)" and
+    H8: "envr xre = Some (VClsr (RecvEvt xrc) envre)" and
+    H9: "envse xsc = Some (VChn c)" and
+    H10: "envre xrc = Some (VChn c)" and 
+    H11: "envse xm = Some vm"
+
+  have H12:
+  "
+    \<forall>\<pi> e \<rho> \<kappa>.
+    \<E>m \<pi> = Some (Stt e \<rho> \<kappa>) \<longrightarrow>
+    staticFlowsAccept V F e \<and> staticFlowsAcceptEnv V F \<rho> \<and> staticFlowsAcceptStack V F  (\<lfloor>e\<rfloor>) \<kappa>"
+  using H1 staticFlowsAcceptPool.cases by blast 
+
+  have H13: "staticFlowsAccept V F (Bind xs (Sync xse) es)"
+    using H12 H4 by blast
+
+  have H14: "staticFlowsAcceptEnv V F envs"
+    using H12 H4 by blast
+
+  have H15: "staticFlowsAcceptStack V F (\<lfloor>Bind xs (Sync xse) es\<rfloor>) ks"
+    using H12 H4 by blast
+
+
+  have H16: "staticFlowsAccept V F (Bind xr (Sync xre) er)"
+  using H12 H7 by blast
+
+  have H17: "staticFlowsAcceptEnv V F envr"
+    using H12 H7 by blast
+
+  have H18: "staticFlowsAcceptStack V F (\<lfloor>Bind xr (Sync xre) er\<rfloor>) kr"
+  using H12 H7 by blast
+
+
+  have H19: "staticFlowsAcceptEnv V F (envs(xs \<mapsto> VUnt))"
+    using H14 staticFlowsAcceptEnv.simps staticFlowsAcceptEnv_staticFlowsAcceptVal.Unit by auto
+
+
+  have H20: "staticFlowsAcceptVal V F (VClsr (SendEvt xsc xm) envse)"
+    using H14 H5 staticFlowsAcceptEnv.cases by blast
+
+  have H21: "staticFlowsAcceptEnv V F envse"
+  using H20 proof cases
+    case SendEvt
+    then show ?thesis by simp
+  qed
+
+  have H22: "staticFlowsAcceptVal V F vm"
+    using H11 H21 staticFlowsAcceptEnv.cases by blast
+
+  have H23: "staticFlowsAcceptEnv V F (envr(xr \<mapsto> vm))"
+    using H11 H17 H21 staticFlowsAcceptEnv.simps by auto
+
+
+  have H24: "staticFlowsAcceptEnv V F (envs(xs \<mapsto> VUnt))"
+    by (simp add: H19)
+
+  have H27: "staticFlowsAccept V F er"
+  using H16 proof cases
+    case BindSync
+    then show ?thesis by simp
+  qed
+
+  have H28: "staticFlowsAccept V F es"
+  using H13 proof cases
+    case BindSync
+    then show ?thesis by simp
+  qed
+
+
+show "staticFlowsAcceptPool V F 
+    (\<E>m(pis @ [LNxt xs] \<mapsto> (Stt es (envs(xs \<mapsto> VUnt)) ks), pir @ [LNxt xr] \<mapsto> (Stt er (envr(xr \<mapsto> vm)) kr)))"
+  using H12 H23 H24 H15 H16 H27 H28 staticFlowsAcceptPool.intros H18 by auto
+qed
+
+lemma staticFlowsAcceptPoolPreservedDynamicEval:
+  "
+  staticFlowsAcceptPool V F \<E>m \<Longrightarrow>
+  (V, C) \<Turnstile>\<^sub>\<E> \<E>m \<Longrightarrow>
+  dynamicEval (\<E>m, Hm) (\<E>', H') \<Longrightarrow>
+  staticFlowsAcceptPool V F \<E>'
+"
+proof -
+  assume 
+    H1: "staticFlowsAcceptPool V F \<E>m" and
+    H2: "(V, C) \<Turnstile>\<^sub>\<E> \<E>m" and
+    H3: "dynamicEval (\<E>m, Hm) (\<E>', H')"
+
+  from H3
+  show "staticFlowsAcceptPool V F \<E>'"
+  proof cases
+    case (Seq_Step_Down pi x env xk ek envk k v)
+    then show ?thesis using H1 H2 staticFlowsAcceptPoolPreservedReturnEval by blast
+  next
+    case (Seq_Step pi x b e env k v)
+    then show ?thesis using H1 H2 staticFlowsAcceptPoolPreservedSeqEval by auto
+  next
+    case (Seq_Step_Up pi x b e env k e' env')
+    then show ?thesis using H1 H2 staticFlowsAcceptPoolPreservedCallEval by blast
+  next
+    case (BindMkChn pi x e env k)
+    then show ?thesis  using H1 H2 staticFlowsAcceptPoolPreservedMkChnEval by blast
+  next
+    case (BindSpawn pi x ec e env k)
+    then show ?thesis using H1 H2 staticFlowsAcceptPoolPreservedSpawnEval by auto
+  next
+    case (BindSync pis xs xse es envs ks xsc xm envse pir xr xre er envr kr xrc envre c vm)
+    then show ?thesis using H1 H2 staticFlowsAcceptPoolPreservedSyncEval by auto
+  qed
+qed
+
+
+lemma staticFlowsAcceptPoolPreserved:
+  "
+  staticFlowsAcceptPool V F [[] \<mapsto> (Stt e0 empty [])] \<Longrightarrow>
+  (V, C) \<Turnstile>\<^sub>e e0 \<Longrightarrow>
+  star dynamicEval ([[] \<mapsto> (Stt e0 empty [])], {}) (\<E>', H') \<Longrightarrow>
+  staticFlowsAcceptPool V F \<E>'
+"
+proof -
+  assume 
+    H1: "staticFlowsAcceptPool V F [[] \<mapsto> (Stt e0 empty [])]" and
+    H2: "(V, C) \<Turnstile>\<^sub>e e0" and
+    H4: "star dynamicEval ([[] \<mapsto> (Stt e0 empty [])], {}) (\<E>', H')"
+
+  obtain EH EH' where
+    H6: "EH = ([[] \<mapsto> (Stt e0 empty [])], {})" and 
+    H7: "EH' = (\<E>', H')" and 
+    H8: "star dynamicEval EH EH'"
+    by (simp add: H4)
+
+  have H9: "star_left dynamicEval EH EH'"
+    by (simp add: H4 H6 H7 star_implies_star_left)
+
+  from H9
+  have 
+    H10:
+  "
+    \<forall> \<E>' H' .
+    ([[] \<mapsto> (Stt e0 empty [])], {}) = EH \<longrightarrow> staticFlowsAcceptPool V F [[] \<mapsto> (Stt e0 empty [])] \<longrightarrow>
+    (\<E>', H') = EH' \<longrightarrow> staticFlowsAcceptPool V F \<E>'" 
+  proof induction
+    case (refl x)
+    then show ?case by blast
+  next
+    case (step x y z)
+    {
+      fix \<E>' H'
+      assume 
+        L1H1: "([[] \<mapsto> (Stt e0 empty [])], {}) = x" and
+        L1H2: "staticFlowsAcceptPool V F [[] \<mapsto> (Stt e0 empty [])]" and
+        L1H3: "(\<E>', H') = z"
+
+      have L1H4 : "(V, C) \<Turnstile>\<^sub>\<E> [[] \<mapsto> (Stt e0 empty [])]" by (simp add: H2 staticEval_to_pool)
+
+      have 
+        L1H6: "\<forall> \<E>m Hm . (\<E>m, Hm) = y \<longrightarrow> (V, C) \<Turnstile>\<^sub>\<E> \<E>m \<longrightarrow> staticFlowsAcceptPool V F \<E>m"
+        using L1H1 L1H2 L1H4 step.IH by blast
+
+      have L1H7: "\<exists> \<E>m Hm . (\<E>m, Hm) = y \<and> (V, C) \<Turnstile>\<^sub>\<E> \<E>m "
+        by (metis L1H1 L1H4 eq_fst_iff star_left_implies_star staticEvalPreserved step.hyps(1))
+
+      have L1H8: "staticFlowsAcceptPool V F \<E>'"
+        using L1H3 L1H6 L1H7 staticFlowsAcceptPoolPreservedDynamicEval step.hyps(2) by auto
+    }
+
+    then show ?case 
+      by blast
+  qed
+
+  show "staticFlowsAcceptPool V F \<E>'"
+    using H1 H10 H2 H6 H7 by blast
+
+qed
+
+lemma staticLiveChanToPool:
+  "
+  staticLiveChan V Ln Lx xC e \<Longrightarrow>
+  staticLiveChanPool V Ln Lx xC [[] \<mapsto> (Stt e empty [])]
+"
+sorry
+
+lemma staticLiveChanPoolPreserved:
+  "
+  staticLiveChanPool V Ln Lx xC [[] \<mapsto> (Stt e0 empty [])] \<Longrightarrow>
+  (V, C) \<Turnstile>\<^sub>e e0 \<Longrightarrow>
+  star dynamicEval ([[] \<mapsto> (Stt e0 empty [])], {}) (\<E>', H') \<Longrightarrow>
+  staticLiveChanPool V Ln Lx xC \<E>'
+"
+sorry
+
+
+
 lemma staticTraceablePoolSound':
   assumes
     H1: "star_left dynamicEval EH EH'" and
@@ -352,6 +1018,30 @@ apply (insert staticTraceablePoolSound'[of "([[] \<mapsto> (Stt e empty [])], {}
 apply auto
 done
 
+lemma staticFlowsAcceptToPool:
+  "
+  staticFlowsAccept V F e \<Longrightarrow>
+  staticFlowsAcceptPool V F [[] \<mapsto> (Stt e empty [])]
+"
+apply (erule staticFlowsAccept.cases; auto)
+  apply (simp add: staticFlowsAccept.Result staticFlowsAcceptEnv.simps staticFlowsAcceptPool.Intro staticFlowsAcceptStack.Empty)
+  apply (simp add: staticFlowsAccept.BindUnit staticFlowsAcceptEnv.simps staticFlowsAcceptPool.intros staticFlowsAcceptStack.Empty)
+  apply (simp add: staticFlowsAccept.BindMkChn staticFlowsAcceptEnv.simps staticFlowsAcceptPool.intros staticFlowsAcceptStack.Empty)
+  apply (simp add: staticFlowsAccept.BindSendEvt staticFlowsAcceptEnv.simps staticFlowsAcceptPool.intros staticFlowsAcceptStack.Empty)
+  apply (simp add: staticFlowsAccept.BindRecvEvt staticFlowsAcceptEnv.simps staticFlowsAcceptPool.intros staticFlowsAcceptStack.Empty)
+  apply (simp add: staticFlowsAccept.BindPair staticFlowsAcceptEnv.simps staticFlowsAcceptPool.intros staticFlowsAcceptStack.Empty)
+  apply (simp add: staticFlowsAccept.BindLeft staticFlowsAcceptEnv.simps staticFlowsAcceptPool.intros staticFlowsAcceptStack.Empty)
+  apply (simp add: staticFlowsAccept.BindRight staticFlowsAcceptEnv.simps staticFlowsAcceptPool.intros staticFlowsAcceptStack.Empty)
+  apply (simp add: staticFlowsAccept.BindFun staticFlowsAcceptEnv.simps staticFlowsAcceptPool.intros staticFlowsAcceptStack.Empty)
+  apply (simp add: staticFlowsAccept.BindSpawn staticFlowsAcceptEnv.simps staticFlowsAcceptPool.intros staticFlowsAcceptStack.Empty)
+  apply (simp add: staticFlowsAccept.BindSync staticFlowsAcceptEnv.simps staticFlowsAcceptPool.intros staticFlowsAcceptStack.Empty)
+  apply (simp add: staticFlowsAccept.BindFst staticFlowsAcceptEnv.simps staticFlowsAcceptPool.intros staticFlowsAcceptStack.Empty)
+  apply (simp add: staticFlowsAccept.BindSnd staticFlowsAcceptEnv.simps staticFlowsAcceptPool.intros staticFlowsAcceptStack.Empty)
+  apply (simp add: staticFlowsAccept.BindCase staticFlowsAcceptEnv.simps staticFlowsAcceptPool.intros staticFlowsAcceptStack.Empty)
+  apply (simp add: staticFlowsAccept.BindApp staticFlowsAcceptEnv.simps staticFlowsAcceptPool.intros staticFlowsAcceptStack.Empty)
+done
+
+
 lemma staticTraceableSound: "
   \<E>' \<pi> = Some (Stt (Bind x b e\<^sub>n) \<rho> \<kappa>) \<Longrightarrow>
   dynamicBuiltOnChanComplex \<rho> (Ch \<pi>C xC) b \<Longrightarrow>
@@ -364,8 +1054,12 @@ lemma staticTraceableSound: "
     pathsCongruentModChan (\<E>', H') (Ch \<pi>C xC) \<pi> path \<and>
     staticTraceable F Ln Lx (IdBind xC) isEnd path
 "
-sorry
-(*  use induction on star_left dynamicEval along with deep definition of staticFlowsAccept *)
+apply (drule staticFlowsAcceptToPool)
+apply (drule staticLiveChanToPool)
+apply (drule staticTraceablePoolSound; auto?)
+apply (erule staticLiveChanPoolPreserved; auto?)
+apply (erule staticFlowsAcceptPoolPreserved; auto?)
+done
 
 lemma sendEvtBuiltOnChan:
 "
